<?xml version="1.0"?>
<rdf:RDF xmlns="http://www.iri.upc.edu/groups/perception/OCRA/ont/ocra_home.owl"
     xml:base="http://www.iri.upc.edu/groups/perception/OCRA/ont/ocra_home.owl"
     xmlns:dc="http://purl.org/dc/elements/1.1/"
     xmlns:DUL="http://www.ontologydesignpatterns.org/ont/dul/DUL.owl#"
     xmlns:owl="http://www.w3.org/2002/07/owl#"
     xmlns:rdf="http://www.w3.org/1999/02/22-rdf-syntax-ns#"
     xmlns:xml="http://www.w3.org/XML/1998/namespace"
     xmlns:xsd="http://www.w3.org/2001/XMLSchema#"
     xmlns:ocra="http://www.iri.upc.edu/groups/perception/OCRA/ont/ocra.owl#"
     xmlns:rdfs="http://www.w3.org/2000/01/rdf-schema#">
    <owl:Ontology rdf:about="http://www.iri.upc.edu/groups/perception/OCRA/ont/ocra_home.owl">
        <owl:imports rdf:resource="http://www.iri.upc.edu/groups/perception/OCRA/ont/ocra.owl"/>
    </owl:Ontology>
    


    <!-- 
    ///////////////////////////////////////////////////////////////////////////////////////
    //
    // Object Properties
    //
    ///////////////////////////////////////////////////////////////////////////////////////
     -->

    


    <!-- http://www.iri.upc.edu/groups/perception/OCRA/ont/ocra_home.owl#hasFlavor -->

    <owl:ObjectProperty rdf:about="http://www.iri.upc.edu/groups/perception/OCRA/ont/ocra_home.owl#hasFlavor">
        <rdfs:subPropertyOf rdf:resource="http://www.ontologydesignpatterns.org/ont/dul/DUL.owl#hasQuality"/>
        <rdfs:comment xml:lang="en">Relationship between Drinks and their flavor(s). 

Note that a drink can have several flavors. Furthermore, this relation can be generalized to hold between other entities and their flavor (e.g., food, dishes, etc.). However, for this application ontology it has been decided to model it only for the objects of interest: drinks.</rdfs:comment>
        <rdfs:label>has flavor</rdfs:label>
    </owl:ObjectProperty>
    


    <!-- http://www.iri.upc.edu/groups/perception/OCRA/ont/ocra_home.owl#hasTemperature -->

    <owl:ObjectProperty rdf:about="http://www.iri.upc.edu/groups/perception/OCRA/ont/ocra_home.owl#hasTemperature">
        <rdfs:subPropertyOf rdf:resource="http://www.ontologydesignpatterns.org/ont/dul/DUL.owl#hasQuality"/>
        <rdfs:comment xml:lang="en">Relationship between Drinks and their Temperature.

Note that this relation can be generalized to hold between other entities and their temperature (e.g., the volume of a room, a car, a city, etc.). However, for this application ontology it has been decided to model it only for the objects of interest: drinks.</rdfs:comment>
        <rdfs:label>has temperature</rdfs:label>
    </owl:ObjectProperty>
    


    <!-- http://www.iri.upc.edu/groups/perception/OCRA/ont/ocra_home.owl#isColderThan -->

    <owl:ObjectProperty rdf:about="http://www.iri.upc.edu/groups/perception/OCRA/ont/ocra_home.owl#isColderThan">
        <rdfs:subPropertyOf rdf:resource="http://www.ontologydesignpatterns.org/ont/dul/DUL.owl#associatedWith"/>
        <owl:inverseOf rdf:resource="http://www.iri.upc.edu/groups/perception/OCRA/ont/ocra_home.owl#isHotterThan"/>
        <rdfs:domain rdf:resource="http://www.iri.upc.edu/groups/perception/OCRA/ont/ocra_home.owl#Drink"/>
        <rdfs:range rdf:resource="http://www.iri.upc.edu/groups/perception/OCRA/ont/ocra_home.owl#Drink"/>
        <rdfs:comment xml:lang="en">Relationship between two Drinks, indicating that one of them has a lower temperature. 

Note that this relation can be generalized to hold between other entities (e.g., two fruits, rooms, cities,  etc.). However, for this application ontology it has been decided to model it only for the objects of interest: drinks.</rdfs:comment>
        <rdfs:label xml:lang="en">is colder than</rdfs:label>
    </owl:ObjectProperty>
    


    <!-- http://www.iri.upc.edu/groups/perception/OCRA/ont/ocra_home.owl#isHotterThan -->

    <owl:ObjectProperty rdf:about="http://www.iri.upc.edu/groups/perception/OCRA/ont/ocra_home.owl#isHotterThan">
        <rdfs:subPropertyOf rdf:resource="http://www.ontologydesignpatterns.org/ont/dul/DUL.owl#associatedWith"/>
        <rdfs:domain rdf:resource="http://www.iri.upc.edu/groups/perception/OCRA/ont/ocra_home.owl#Drink"/>
        <rdfs:range rdf:resource="http://www.iri.upc.edu/groups/perception/OCRA/ont/ocra_home.owl#Drink"/>
        <rdfs:comment xml:lang="en">Relationship between two Drinks, indicating that one has a higher temperature than the other one.  

Note that this relation can be generalized to hold between other entities (e.g., two fruits, rooms, cities,  etc.). However, for this application ontology it has been decided to model it only for the objects of interest: drinks.</rdfs:comment>
        <rdfs:label xml:lang="en">is hotter than</rdfs:label>
    </owl:ObjectProperty>
    


    <!-- http://www.iri.upc.edu/groups/perception/OCRA/ont/ocra_home.owl#isLessTastyThan -->

    <owl:ObjectProperty rdf:about="http://www.iri.upc.edu/groups/perception/OCRA/ont/ocra_home.owl#isLessTastyThan">
        <rdfs:subPropertyOf rdf:resource="http://www.ontologydesignpatterns.org/ont/dul/DUL.owl#associatedWith"/>
        <owl:inverseOf rdf:resource="http://www.iri.upc.edu/groups/perception/OCRA/ont/ocra_home.owl#isTastierThan"/>
        <rdfs:domain rdf:resource="http://www.iri.upc.edu/groups/perception/OCRA/ont/ocra_home.owl#Drink"/>
        <rdfs:range rdf:resource="http://www.iri.upc.edu/groups/perception/OCRA/ont/ocra_home.owl#Drink"/>
        <rdfs:comment xml:lang="en">Relationship between two Drinks, indicating that one is less tasty that the other one. 

Note that this relation can be generalized to hold between other entities (e.g., two fruits, dishes,  etc.). However, for this application ontology it has been decided to model it only for the objects of interest: drinks.</rdfs:comment>
        <rdfs:label xml:lang="en">is less tasty than</rdfs:label>
    </owl:ObjectProperty>
    


    <!-- http://www.iri.upc.edu/groups/perception/OCRA/ont/ocra_home.owl#isMoreNaturalThan -->

    <owl:ObjectProperty rdf:about="http://www.iri.upc.edu/groups/perception/OCRA/ont/ocra_home.owl#isMoreNaturalThan">
        <rdfs:subPropertyOf rdf:resource="http://www.ontologydesignpatterns.org/ont/dul/DUL.owl#associatedWith"/>
        <owl:inverseOf rdf:resource="http://www.iri.upc.edu/groups/perception/OCRA/ont/ocra_home.owl#isMoreProcessedThan"/>
        <rdfs:domain rdf:resource="http://www.iri.upc.edu/groups/perception/OCRA/ont/ocra_home.owl#Drink"/>
        <rdfs:range rdf:resource="http://www.iri.upc.edu/groups/perception/OCRA/ont/ocra_home.owl#Drink"/>
        <rdfs:comment xml:lang="en">Relationship between two Drinks, indicating that one has gone through less manufacturing processes until the state in which they are. It is closer to its state found in Nature.  

Note that this relation can be generalized to hold between other entities (e.g., two dishes, cloths,  etc.). However, for this application ontology it has been decided to model it only for the objects of interest: drinks.</rdfs:comment>
        <rdfs:label xml:lang="en">is more natural than</rdfs:label>
    </owl:ObjectProperty>
    


    <!-- http://www.iri.upc.edu/groups/perception/OCRA/ont/ocra_home.owl#isMoreProcessedThan -->

    <owl:ObjectProperty rdf:about="http://www.iri.upc.edu/groups/perception/OCRA/ont/ocra_home.owl#isMoreProcessedThan">
        <rdfs:subPropertyOf rdf:resource="http://www.ontologydesignpatterns.org/ont/dul/DUL.owl#associatedWith"/>
        <rdfs:domain rdf:resource="http://www.iri.upc.edu/groups/perception/OCRA/ont/ocra_home.owl#Drink"/>
        <rdfs:range rdf:resource="http://www.iri.upc.edu/groups/perception/OCRA/ont/ocra_home.owl#Drink"/>
        <rdfs:comment xml:lang="en">Relationship between two Drinks, indicating that one of them has gone through more manufacturing processes until its current state. 

Note that this relation can be generalized to hold between other entities (e.g., two fruits, dishes,  etc.). However, for this application ontology it has been decided to model it only for the objects of interest: drinks.</rdfs:comment>
        <rdfs:label xml:lang="en">is more processed than</rdfs:label>
    </owl:ObjectProperty>
    


    <!-- http://www.iri.upc.edu/groups/perception/OCRA/ont/ocra_home.owl#isTastierThan -->

    <owl:ObjectProperty rdf:about="http://www.iri.upc.edu/groups/perception/OCRA/ont/ocra_home.owl#isTastierThan">
        <rdfs:subPropertyOf rdf:resource="http://www.ontologydesignpatterns.org/ont/dul/DUL.owl#associatedWith"/>
        <rdfs:domain rdf:resource="http://www.iri.upc.edu/groups/perception/OCRA/ont/ocra_home.owl#Drink"/>
        <rdfs:range rdf:resource="http://www.iri.upc.edu/groups/perception/OCRA/ont/ocra_home.owl#Drink"/>
        <rdfs:comment xml:lang="en">Relationship between two Drinks, indicating that one is tastier than the other one.  

Note that this relation can be generalized to hold between other entities (e.g., two fruits, dishes,  etc.). However, for this application ontology it has been decided to model it only for the objects of interest: drinks.</rdfs:comment>
        <rdfs:label xml:lang="en">is tastier than</rdfs:label>
    </owl:ObjectProperty>
    


    <!-- 
    ///////////////////////////////////////////////////////////////////////////////////////
    //
    // Classes
    //
    ///////////////////////////////////////////////////////////////////////////////////////
     -->

    


    <!-- http://www.iri.upc.edu/groups/perception/OCRA/ont/ocra_home.owl#Drink -->

    <owl:Class rdf:about="http://www.iri.upc.edu/groups/perception/OCRA/ont/ocra_home.owl#Drink">
        <rdfs:subClassOf rdf:resource="http://www.ontologydesignpatterns.org/ont/dul/DUL.owl#Object"/>
        <rdfs:comment xml:lang="en">An Ojbect that refers to a general conceptualization of (an amount of) liquid that is (or can be) taken into the body through the mouth. 

This class can be used to represent both a physical object (e.g. a cup of tea), and a social object referring to the physical one (e.g. would you like to have a tea?).</rdfs:comment>
        <rdfs:label xml:lang="en">Drink</rdfs:label>
    </owl:Class>
</rdf:RDF>



<!-- Generated by the OWL API (version 4.5.6.2018-09-06T00:27:41Z) https://github.com/owlcs/owlapi -->

